nameless-w/Typing.v
@@ -1,11 +1,42 @@
 Require Import Prelude.
 Require Import Expr.
+Require Import Scoping.
+Hint Resolve leP ltP eqP.
+
+Fixpoint map_with_ix {A B} (f : nat -> A -> B) (xs : seq A) : seq B :=
+  match xs with
+      [] => []
+    | x :: xs' => f 0 x :: map_with_ix (fun n a => f n.+1 a) xs'
+  end.
+
+Lemma map_with_ix_funext {A B} xs : forall (f g : nat -> A -> B), (forall n a, f n a = g n a) -> map_with_ix f xs = map_with_ix g xs.
+  induction xs; intros; simpl; f_equal; auto. Qed.
+Hint Rewrite @map_with_ix_funext using solve [eauto].
+Hint Rewrite @iterate_S @iterate_0.
+
+Ltac bdestruct X :=
+  let H := fresh in 
+  let e := fresh "e" in
+  evar (e: Prop); assert (H: reflect e X); subst e;
+  [eauto
+  | destruct H as [H|H]].
+
+Require Import Omega.
+
+Lemma reflect_iff P p : reflect P p -> p <-> P. destruct 1; split; auto; congruence. Qed.
+Hint Rewrite reflect_iff using solve [eauto] : bprop.
+Hint Rewrite <- reflect_iff using solve [eauto] : unprop.
+Ltac conv_to_prop := autorewrite with bprop in *.
+Ltac conv_from_prop := autorewrite with unprop in *.
+
+Goal forall x y z, x < y -> y < z -> x < z. intros. conv_to_prop. omega. Qed.
 
 Notation env a := (Expr.name -> option a).
 Variable (const_tys : env exp).
 Variable (conv : relation exp).
 
-Fixpoint dget {T} `{Ids T} `{Subst T} (Gamma : list T) (n : var) {struct n} : T :=
+(* Notation dget Gamma n := (nth (ids 0) Gamma n).[wk n.+1]. *)
+Fixpoint dget {T} `{Ids T} `{Subst T} (Gamma : seq T) (n : var) {struct n} : T :=
   match Gamma, n with
     | [::], _ => ids 0
     | A :: _, 0 => A.[wk 1]
@@ -21,7 +52,7 @@ Definition imax (i j : nat) := match j with 0 => 0 | _ => max i j end.
 
 (* Fixpoint has_type (Gamma : list exp) (e T : exp) : Prop *)
 (*   match e,T with *)
-(*     | Bind i,_ => (i < length Gamma) /\ (dget Gamma i = T) *)
+(*     | Bind i,_ => (i < size Gamma) /\ (dget Gamma i = T) *)
 (*     | Free nm,_ => const_tys nm = Some *)
 (*     | Sort i, Sort j => i < j *)
 (*     | (A :>> B), Sort k => exists i j, [Gamma |+ A :< Sort i] /\ [A :: Gamma |+ B :< Sort j] /\ imax i j < k *)
@@ -30,8 +61,8 @@ Definition imax (i j : nat) := match j with 0 => 0 | _ => max i j end.
 (*   end *)
 (* where "[ C |+ e :< t ]" := (has_type C e T). *)
 
-Inductive has_type (Gamma : list exp) : exp ->  exp -> Prop :=
-  T_bind : forall i, i < length Gamma -> [Gamma |+ Bind i :< dget Gamma i]
+Inductive has_type (Gamma : seq exp) : exp ->  exp -> Prop :=
+  T_bind : forall i, i < size Gamma -> [Gamma |+ Bind i :< dget Gamma i]
 | T_free : forall nm t, const_tys nm = Some t -> [Gamma |+ Free nm :< t]
 | T_sort : forall s, [Gamma |+ Sort s :< Sort s.+1]
 | T_cumu : forall i j, [Gamma |+ i :< Sort j] -> [Gamma |+ i :< Sort j.+1]
@@ -64,22 +95,22 @@ Inductive has_type (Gamma : list exp) : exp ->  exp -> Prop :=
 | T_mu : forall D C a d, 
          forall n, [(Mu D :: Gamma) |+ C :< Sort n] ->
            (* [(Mu D :: Gamma) |+ C] -> *)
-              [Gamma   |+ a :< (D_efunc D (Mu D) :>> All D C.[up (wk 1)] (Bind 0) :>> C.[Bind 1 .: wk 2])] ->
+              [Gamma   |+ a :< (Mu D :>> (All D C.[up (wk 1)] (Bind 0) :>> C.[Bind 1 .: wk 2]))] ->
               [Gamma   |+ d :< Mu D] ->
               [Gamma   |+ mu D a d :< C.[d/]]
 
 | T_conv : forall A A', conv A A' -> forall a, [Gamma |+ a :< A] -> [Gamma |+ a :< A']
 where "[ C |+ e :< t ]" := (has_type C e t).
 
-Fixpoint has_type_rec (Gamma : list exp) (e : exp) (T : exp) : Prop :=
-  match e with
-    | Bind i => (i < ⟦Gamma⟧) /\ conv T (dget Gamma i)
-    | Free nm => exists t, const_tys nm = Some t /\ conv T t
-    | Sort i => exists j, i < j /\ conv T (Sort j)
-    | A :>> B => exists i j k, has_type_rec Gamma A (Sort i) /\ has_type_rec (A :: Gamma) B (Sort j) /\ k > imax i j /\ conv T (Sort k)
-    | Lam b => exists A B, has_type_rec (A :: Gamma) b B /\ conv T (A :>> B)
-    | _ => False
-  end.
+(* Fixpoint has_type_rec (Gamma : list exp) (e : exp) (T : exp) : Prop := *)
+(*   match e with *)
+(*     | Bind i => (i < ⟦Gamma⟧) /\ conv T (dget Gamma i) *)
+(*     | Free nm => exists t, const_tys nm = Some t /\ conv T t *)
+(*     | Sort i => exists j, i < j /\ conv T (Sort j) *)
+(*     | A :>> B => exists i j k, has_type_rec Gamma A (Sort i) /\ has_type_rec (A :: Gamma) B (Sort j) /\ k > imax i j /\ conv T (Sort k) *)
+(*     | Lam b => exists A B, has_type_rec (A :: Gamma) b B /\ conv T (A :>> B) *)
+(*     | _ => False *)
+(*   end. *)
 (* with is_type (Gamma : list exp) : exp -> Prop := *)
 (*   T_typ : forall e, [Gamma |+ e :< Typ] -> [Gamma |+ e] *)
 (* | T_pi : forall A B, [Gamma |+ A] -> [(A :: Gamma) |+ B] -> [Gamma |+ Pi A B] *)
@@ -90,7 +121,176 @@ Fixpoint has_type_rec (Gamma : list exp) (e : exp) (T : exp) : Prop :=
 
 Notation "[ Delta |+ sigma +| Gamma ]" := (forall x, x < size Gamma -> [Delta |+ sigma x :< (dget Gamma x).[sigma]]) (at level 20).
 
-Lemma sub_cons_typed sigma e E Gamma Delta : [Delta |+ sigma +| Gamma] -> 
+Lemma sub_cons_var sigma e E Gamma Delta : [Delta |+ sigma +| Gamma] -> 
                                              [Delta |+ e :< E.[sigma]] -> 
                                              [Delta |+ e .: sigma +| E :: Gamma].
 Proof. intros; destruct x; asimpl; eauto. Qed.
+
+Hint Constructors has_type.
+Lemma sub_id_ref : forall Gamma, [Gamma |+ ids +| Gamma]. intros; asimpl; auto. Qed.
+Lemma sub_wk_var : forall Gamma A, [A :: Gamma |+ wk 1 +| Gamma]. intros; asimpl; constructor; auto. Qed.
+
+Hint Resolve sub_id_ref sub_wk_var sub_cons_var.
+
+Lemma dget_nth : forall Gamma n, n <  size Gamma -> dget Gamma n = (nth (ids 0) Gamma n).[wk n.+1].
+  induction Gamma; simpl.
+  { inversion 1. }
+  { intros. destruct n; simpl; auto. 
+    rewrite IHGamma; autosubst. }
+Qed.
+  
+Functional Scheme sub_ind := Induction for minus Sort Prop.
+
+Notation ren_scop xi i j := (forall v, v < i -> xi v < j).
+
+Lemma All_sub D : forall sigma C e, (All D C e).[sigma] = All D C.[up sigma] e.[sigma].
+  induction D; intros; simpl; rewrite asms; 
+  try replace C.[up (wk 1)].[up (up sigma)] with C.[up sigma].[up (wk 1)]; autosubst. Qed.
+
+Hint Resolve All_sub.
+Hint Rewrite All_sub.
+
+
+Lemma ty_renaming xi Gamma Delta a A :
+  [ Gamma |+ a :< A ] ->
+  ren_scop xi (size Gamma) (size Delta) ->
+  (forall v, v < size Gamma -> (dget Gamma v).[ren xi] = dget Delta (xi v)) ->
+  [ Delta |+ a.[ren xi] :< A.[ren xi]].
+Proof. move=>Ha; move:xi Delta; induction Ha; simpl; intros; try solve[eauto].
+       { rewrite H1; auto. }
+       { admit. }                (* needs closure properties for env *)
+       { asimpl. constructor; try solve[eauto].
+         apply IHHa2; intros; simpl in *; auto.
+         destruct v; simpl; solve[eauto].
+         destruct v; asimpl; auto.
+         rewrite <- H0; autosubst. }
+       { asimpl. constructor; try solve[eauto].
+         apply IHHa; intros; simpl in *; auto.
+         destruct v; simpl; solve[eauto].
+         destruct v; asimpl; auto.
+         rewrite <- H0; autosubst. }
+       { replace B.[a/].[ren xi] with B.[up (ren xi)].[a.[ren xi]/] by autosubst.
+         econstructor; solve[eauto]. }
+       { asimpl. constructor; try solve[eauto].
+         apply IHHa2; intros; simpl in *; auto.
+         destruct v; simpl; solve[eauto].
+         destruct v; asimpl; auto.
+         rewrite <- H0; autosubst. }
+       { asimpl; constructor; auto.
+         replace B.[ren (upren xi)].[a.[ren xi]/] with B.[a/].[ren xi] by autosubst; solve[eauto]. }
+       { replace B.[S_p1 s/].[ren xi] with B.[up (ren xi)].[S_p1 s.[ren xi]/] by autosubst.
+         apply T_p2 with (A := A.[ren xi]); auto. apply IHHa; auto. }
+       { asimpl.
+         replace P.[ab.[ren xi] .: ren xi] with P.[ren (upren xi)].[ab.[ren xi]/] by autosubst.
+         apply T_split with (A := A.[ren xi]) (B := B.[ren xi]);
+         match goal with [|- context[P.[?x].[?t .: ?r]]] => 
+                         replace P.[x].[t .: r] with P.[t .: r].[x] by autosubst end.
+         { apply IHHa1; intros; destruct v; simpl in *; auto.
+           - apply H; auto.
+           - replace A.[wk 1].[ren (upren xi)] with A.[ren xi].[wk 1] by autosubst; reflexivity.
+           - rewrite <- H0; autosubst. }
+         { apply IHHa2; intros; destruct v; simpl in *; auto.
+           - apply H; auto.
+           - replace B.[wk 1].[ren (upren xi)] with B.[ren xi].[wk 1] by autosubst; reflexivity.
+           - rewrite <- H0; autosubst. } }
+       { replace C.[d/].[ren xi] with C.[ren (upren xi)].[d.[ren xi]/] by autosubst.
+         specialize (IHHa1 (upren xi) (Mu D :: Delta)). specialize (IHHa2 xi Delta H H0). specialize (IHHa3 xi Delta H H0).
+         simpl in *. rewrite All_sub in IHHa2.
+         econstructor; auto.
+         - apply IHHa1; auto; destruct v; simpl in *; intros; auto; apply H || rewrite <- H0; autosubst.           
+         - asimpl; asimpl in IHHa2; exact IHHa2. }
+       { admit. }               (* needs conv sub props *)
+Admitted.
+(* CURRENT POINT *)
+Lemma wk_i_up_jk : forall i j k, sub_eq (wk i >> upn j (wk k)) (upn (j - i) (wk k) >> wk i).
+  intros i j.
+  refine (sub_ind (fun j i ij => forall k, sub_eq (wk i >> upn j (wk k)) (upn ij (wk k) >> wk i)) _ _ _ j i); 
+    intros; subst.
+  { asimpl; f_equal; omega. }
+  { autosubst. }
+  { replace ((wk l.+1 >> upn k.+1 (wk k0)) v) with ((wk l >> upn k (wk k0)) v).[wk 1] by autosubst.
+    rewrite H; autosubst. }
+Qed.
+
+Hint Resolve wk_i_up_jk.
+
+(* Hint Rewrite sub_vars_tms using solve[eauto]. *)
+
+Lemma closed_upn : forall i j sigma, closed_sub j sigma -> closed_sub (i + j) (upn i sigma).
+  induction i; move=>j sigma; rewrite ?iterate_S; solve[eauto]. Qed.
+
+Hint Resolve closed_upn.
+
+Lemma wk_ty A Gamma e T : [Gamma |+ e :< T] -> [A :: Gamma |+ e.[wk 1] :< T.[wk 1]]. intros; apply ty_renaming with (Gamma := Gamma); auto. Qed.
+Hint Resolve wk_ty.
+
+Lemma up_ty A Gamma Delta sigma : [Gamma |+ sigma +| Delta] -> [A.[sigma] :: Gamma |+ up sigma +| A :: Delta].
+Proof. destruct x; simpl; intros; auto; asimpl; rewrite <- subst_comp; try constructor; auto. Qed.
+Hint Resolve up_ty.
+
+Hint Extern 1 (_.[_] = _.[_]) => autosubst.
+
+Lemma sub_var_cor : forall e Delta T, [Delta |+ e :< T] -> forall sigma Gamma, [Gamma |+ sigma +| Delta] -> [Gamma |+ e.[sigma] :< T.[sigma]].
+Proof. induction 1; simpl; intros; auto;
+  asimpl; rewrite <- ?subst_comp;
+  try solve [eauto].
+  { admit. }               (* free vars need closure properties *)
+  { replace B.[a.[sigma] .: sigma] with B.[up sigma].[a.[sigma]/]; solve[eauto]. }
+  { econstructor; try replace B.[up sigma].[a.[sigma]/] with B.[a/].[sigma]; solve[auto]. }
+  { replace B.[S_p1 s.[sigma] .: sigma] with B.[up sigma].[S_p1 s.[sigma]/]; solve[eauto]. }
+  { replace P.[ab.[sigma] .: sigma] with P.[up sigma].[ab.[sigma]/] by autosubst. 
+    econstructor. 
+    { specialize (IHhas_type1 (up sigma)). asimpl in *. auto. }
+    { specialize (IHhas_type2 (up sigma)). asimpl in *. auto. } }
+  { replace C.[d.[sigma] .: sigma] with C.[up sigma].[d.[sigma]/]; auto. econstructor; try solve[eauto].
+    { eapply IHhas_type1. destruct x; intros.
+      { asimpl. constructor; auto. }
+      { asimpl; rewrite <- subst_comp; auto. } }
+    { replace C.[up sigma].[Bind 1 .: wk 2] with C.[Bind 1 .: wk 2].[up (up sigma)] by autosubst.
+      replace C.[up sigma].[up (wk 1)] with C.[up (wk 1)].[up (up sigma)] by autosubst.
+      replace (Mu D :>> (All D C.[up (wk 1)].[up (up sigma)] (Bind 0) :>> C.[Bind 1 .: wk 2].[up (up sigma)]))
+      with (Mu D :>> (All D C.[up (wk 1)] (Bind 0) :>> C.[Bind 1 .: wk 2]).[up sigma]) 
+        by (asimpl; rewrite All_sub; autosubst).
+      eauto. } }
+  { admit. }               (* conv property *)
+Admitted.
+
+Hint Resolve sub_var_cor.
+(* Notation "x .[ sigma ]" := (map (fun y => y.[sigma]) x). *)
+Hint Rewrite <- subst_comp.
+
+Lemma sub_comp_cor Gamma Delta Sigma delta sigma : [Gamma |+ delta +| Delta] -> [Delta |+ sigma +| Sigma] -> [Gamma |+ sigma >> delta +| Sigma].
+Proof. intros; asimpl; autorewrite with core; solve[eauto]. Qed.
+
+Require Import Reduction.
+
+Notation conv_con Gamma Delta := (size Gamma = size Delta /\ forall i, conv (dget Delta i) (dget Gamma i)). 
+
+Hypothesis step_conv : forall e e', e ::> e' -> conv e e'.
+Hypothesis step_back_conv : forall e e', e ::> e' -> conv e' e.
+Hypothesis conv_refl : forall e, conv e e.
+Hypothesis conv_trans : forall e e' e'', conv e e' -> conv e' e'' -> conv e e''.
+Hypothesis conv_symm : forall e e', conv e e' -> conv e' e.
+Hypothesis conv_sub_congr1 : forall e e' sigma, conv e e' -> conv e.[sigma] e'.[sigma].
+Hypothesis conv_sub_congr : forall e e' sigma tau, sigma .>> tau -> conv e.[sigma] e'.[tau].
+Hint Resolve conv_refl conv_sub_congr1.
+Hint Resolve step_conv.
+
+Lemma lam_pi Gamma A B b : [Gamma |+ Lam b :< A :>> B] -> [A :: Gamma |+ b :< B].
+Proof. remember (Lam b) as lb; remember (A :>> B) as ab.
+  induction 1; inversion Heqlb; inversion Heqab; subst; auto.
+(* Hint Extern 1 (conv (dget (?A :: ?Delta) ?i) (dget (?A' :: ?Gamma) ?i)) => destruct i; simpl. *)
+Theorem preservation Gamma Delta e e' T : conv_con Gamma Delta -> e ::> e' -> [Gamma |+ e :< T] -> [Delta |+ e' :< T].
+Proof. move=>Hgd He' He. move: e' He' Delta Hgd. 
+  induction He; simpl; intros; destruct Hgd as [Hl Hi]; inverts He'; try (try econstructor; solve[eauto]).
+  Local Hint Extern 1 (conv (dget (?A :: ?Delta) ?i) (dget (?A' :: ?Gamma) ?i)) => destruct i; simpl.
+  Hint Resolve step_back_conv.
+  { constructor. apply IHHe1; auto. apply IHHe2; auto; simpl; split; auto. }
+  { constructor. apply IHHe1; auto. apply IHHe2; auto. simpl; split; auto. }
+  { constructor. apply IHHe; auto. simpl; split; auto. }
+  { constructor. apply IHHe; auto. simpl; split; auto. }
+  { apply T_conv with (A := B.[a'/]); auto. apply T_app with (A := A); auto. }
+  { apply T_conv with (A := B.[a'/]); auto. 
+    assert (H: [Delta |+ Lam b :< (A :>> B)]) by auto.
+    - eapply sub_var_cor; try eassumption. inversion H; subst; try eassumption. 
+    - 
